Optimizations/Canonicalizations/Common.thy
@@ -7,18 +7,59 @@ theory Common
 begin
 
 lemma size_pos[size_simps]: "0 < size y"
-  by (induction y; auto?)
+  apply (induction y; auto?)
+  by (smt (z3) add_2_eq_Suc' add_is_0 not_gr0 size.elims size.simps(12) size.simps(13) size.simps(14) size.simps(15) zero_neq_numeral zero_neq_one)
 
-lemma size_non_add[size_simps]: "size (BinaryExpr op a b) = size a + (size b) * 2"
-  by (induction op; auto)
+lemma size_non_add[size_simps]: "size (BinaryExpr op a b) = size a + size b + 2 \<longleftrightarrow> \<not>(is_ConstantExpr b)"
+  by (induction b; induction op; auto simp: is_ConstantExpr_def)
 
 lemma size_non_const[size_simps]:
   "\<not> is_ConstantExpr y \<Longrightarrow> 1 < size y"
   using size_pos apply (induction y; auto)
-  apply (metis Suc_lessI mult_eq_1_iff mult_pos_pos n_not_Suc_n numeral_2_eq_2 pos2)
-  by (metis add_strict_increasing less_Suc0 linorder_not_less mult_2_right not_add_less2)
+  by (metis Suc_lessI add_is_1 is_ConstantExpr_def le_less linorder_not_le n_not_Suc_n numeral_2_eq_2 pos2 size.simps(2) size_non_add)
 
-lemmas arith[size_simps] = Suc_leI add_strict_increasing
+lemma size_binary_const[size_simps]:
+  "size (BinaryExpr op a b) = size a + 2 \<longleftrightarrow> (is_ConstantExpr b)"
+  by (induction b; auto simp: is_ConstantExpr_def size_pos)
+
+lemma size_flip_binary[size_simps]:
+  "\<not>(is_ConstantExpr y) \<longrightarrow> size (BinaryExpr op (ConstantExpr x) y) > size (BinaryExpr op y (ConstantExpr x))"
+  by (metis add_Suc not_less_eq order_less_asym plus_1_eq_Suc size.simps(11) size.simps(2) size_non_add)
+
+lemma size_binary_lhs_a[size_simps]:
+  "size (BinaryExpr op (BinaryExpr op' a b) c) > size a"
+  by (metis add_lessD1 less_add_same_cancel1 pos2 size_binary_const size_non_add)
+
+lemma size_binary_lhs_b[size_simps]:
+  "size (BinaryExpr op (BinaryExpr op' a b) c) > size b"
+  by (metis IRExpr.disc(42) One_nat_def add.left_commute add.right_neutral is_ConstantExpr_def less_add_Suc2 numeral_2_eq_2 plus_1_eq_Suc size.simps(11) size_binary_const size_non_add size_non_const trans_less_add1)
+
+lemma size_binary_lhs_c[size_simps]:
+  "size (BinaryExpr op (BinaryExpr op' a b) c) > size c"
+  by (metis IRExpr.disc(42) add.left_commute add.right_neutral is_ConstantExpr_def less_Suc_eq numeral_2_eq_2 plus_1_eq_Suc size.simps(11) size_non_add size_non_const trans_less_add2)
+
+lemma size_binary_rhs_a[size_simps]:
+  "size (BinaryExpr op c (BinaryExpr op' a b)) > size a"
+  by (smt (verit, best) less_Suc_eq less_add_Suc2 less_add_same_cancel1 linorder_neqE_nat not_add_less1 order_less_trans pos2 size.simps(4) size_binary_const size_non_add)
+
+
+lemma size_binary_rhs_b[size_simps]:
+  "size (BinaryExpr op c (BinaryExpr op' a b)) > size b"
+  by (metis add.left_commute add.right_neutral is_ConstantExpr_def lessI numeral_2_eq_2 plus_1_eq_Suc size.simps(11) size.simps(4) size_non_add trans_less_add2)
+
+lemma size_binary_rhs_c[size_simps]:
+  "size (BinaryExpr op c (BinaryExpr op' a b)) > size c"
+  by simp
+
+lemma size_binary_lhs[size_simps]:
+  "size (BinaryExpr op x y) > size x"
+  by (metis One_nat_def Suc_eq_plus1 add_Suc_right less_add_Suc1 numeral_2_eq_2 size_binary_const size_non_add)
+
+lemma size_binary_rhs[size_simps]:
+  "size (BinaryExpr op x y) > size y"
+  by (metis IRExpr.disc(42) add_strict_increasing is_ConstantExpr_def linorder_not_le not_add_less1 size.simps(11) size_non_add size_non_const size_pos)
+
+lemmas arith[size_simps] = Suc_leI add_strict_increasing order_less_trans trans_less_add2
 
 definition well_formed_equal :: "Value \<Rightarrow> Value \<Rightarrow> bool" 
   (infix "\<approx>" 50) where
